Using ifoldl to avoid some deep copies

PAC_Checker_LLVM/Interleaving_Fold.thy
@@ -226,9 +226,6 @@ proof -
     by (sepref_to_hoare; vcg)
 qed
 
-text \<open>Refinement of the monadic fold @{term foldl_nres}: the step function is an
-  \<open>nres\<close> program, so its rule carries a \<open>nofail\<close> premise and a refinement
-  postcondition (the shape of @{thm hn_refineD}).\<close>
 lemma cl_fold_monadic'_nres_rule:
   assumes F: \<open>\<And>a ai b bi. nofail (f a b) \<Longrightarrow> llvm_htriple
     (A a ai ** B b bi) (fi ai bi)
@@ -258,9 +255,6 @@ next
     by vcg
 qed
 
-text \<open>Variant with the \<open>nofail\<close> condition in the precondition. As a rule premise
-  it is checked before the pure parts of the current state are extracted, which
-  loses facts such as \<open>drop j cs = []\<close> obtained from \<open>cl_assn' C (drop j cs) null\<close>.\<close>
 lemma cl_fold_monadic'_nres_rule':
   assumes F: \<open>\<And>a ai b bi. nofail (f a b) \<Longrightarrow> llvm_htriple
     (A a ai ** B b bi) (fi ai bi)
@@ -479,19 +473,19 @@ qed
 
 context begin
 
-private lemma cl_assn'_cong_fri:
+lemma cl_assn'_cong_fri:
   \<open>PRECOND (SOLVE_AUTO (a = a')) \<Longrightarrow> cl_assn' A a c \<turnstile> cl_assn' A a' c\<close>
   unfolding vcg_tag_defs by simp
 
-private lemma olseg_empty_fri:
+lemma olseg_empty_fri:
   \<open>PRECOND (SOLVE_AUTO (ys = [] \<and> p = q)) \<Longrightarrow> \<box> \<turnstile> olseg A ys p q\<close>
   unfolding vcg_tag_defs by (simp add: olseg_nil sep_algebra_simps)
 
-private lemma olseg_cl_fri:
+lemma olseg_cl_fri:
   \<open>PRECOND (SOLVE_AUTO (ys = xs)) \<Longrightarrow> olseg A ys p null \<turnstile> cl_assn' A xs p\<close>
   unfolding vcg_tag_defs by (simp add: cl_assn_olseg)
 
-private lemma drop_head:
+lemma drop_head:
   \<open>i < length xs \<Longrightarrow> drop i xs = xs ! i # drop (Suc i) xs\<close>
   by (simp add: Cons_nth_drop_Suc)
 
@@ -674,8 +668,6 @@ lemma cl_ifoldl_nres_hfref:
          hfref_nres_htriple_d1_k2[OF F1] hfref_nres_htriple_d1_k2[OF F2]]
   by (sepref_to_hoare; vcg)
 
-text \<open>The functional variant follows by monotonicity of \<open>hfref\<close> in the
-  abstract program, via @{thm ifoldl_nres_refine}.\<close>
 lemma cl_ifoldl_hfref:
   assumes F: \<open>(uncurry3 fi, uncurry3 (RETURN oooo f))
       \<in> A\<^sup>d *\<^sub>a B\<^sup>k *\<^sub>a C\<^sup>k *\<^sub>a dir_assn\<^sup>k \<rightarrow>\<^sub>a A\<close>
@@ -721,6 +713,372 @@ lemma dir_eq_hnr[sepref_fr_rules]:
   supply [vcg_rules] = ll_icmp_eq_bool_rule
   supply [simp] = pure_def bool1_rel_def bool.rel_def in_br_conv
   by (sepref_to_hoare; vcg)
+
+section \<open>Extending to additional types\<close>
+text \<open>In some cases, additional types might be required in f, dec functions
+  (e.g. addition function in shared checker requires the variable lookup table
+   therefore we extend the ifoldl to allow threading additional types)\<close>
+
+fun ifoldl_ext :: \<open>('a \<Rightarrow> 'b \<Rightarrow> 'c \<Rightarrow> 'd \<Rightarrow> direction \<Rightarrow> 'a) \<Rightarrow> ('b \<Rightarrow> 'c \<Rightarrow> 'd \<Rightarrow> direction)
+  \<Rightarrow> ('a \<Rightarrow> 'b \<Rightarrow> 'a) \<Rightarrow> ('a \<Rightarrow> 'c \<Rightarrow> 'a)
+  \<Rightarrow> 'a \<Rightarrow> 'b list \<Rightarrow> 'c list \<Rightarrow> 'd \<Rightarrow> 'a\<close> where
+  \<open>ifoldl_ext _ _   _  _  acc [] [] _             = acc\<close>
+| \<open>ifoldl_ext _ _   f1 _  acc xs [] _             = foldl f1 acc xs\<close>
+| \<open>ifoldl_ext _ _   _  f2 acc [] ys _             = foldl f2 acc ys\<close>
+| \<open>ifoldl_ext f dec f1 f2 acc (x # xs) (y # ys) d = (
+    case dec x y d of
+      STOP  \<Rightarrow> (f acc x y d STOP)
+    | LEFT  \<Rightarrow> ifoldl_ext f dec f1 f2 (f acc x y d LEFT)  xs (y # ys) d
+    | RIGHT \<Rightarrow> ifoldl_ext f dec f1 f2 (f acc x y d RIGHT) (x # xs) ys d
+    | BOTH  \<Rightarrow> ifoldl_ext f dec f1 f2 (f acc x y d BOTH)  xs ys d
+  )\<close>
+
+lemma ifoldl_ext_Nil2: \<open>ifoldl_ext f dec f1 f2 acc xs [] d = foldl f1 acc xs\<close>
+  by (cases xs) auto
+
+lemma ifoldl_ext_Nil1: \<open>ifoldl_ext f dec f1 f2 acc [] ys d = foldl f2 acc ys\<close>
+  by (cases ys) auto
+
+subsection \<open>Monadic version of @{term ifoldl_ext}\<close>
+
+definition ifoldl_ext_nres ::
+  \<open>('a \<Rightarrow> 'b \<Rightarrow> 'c \<Rightarrow> 'd \<Rightarrow> direction \<Rightarrow> 'a nres) \<Rightarrow> ('b \<Rightarrow> 'c \<Rightarrow> 'd \<Rightarrow> direction nres)
+  \<Rightarrow> ('a \<Rightarrow> 'b \<Rightarrow> 'a nres) \<Rightarrow> ('a \<Rightarrow> 'c \<Rightarrow> 'a nres)
+  \<Rightarrow> 'a \<Rightarrow> 'b list \<Rightarrow> 'c list \<Rightarrow> 'd \<Rightarrow> 'a nres\<close> where
+  \<open>ifoldl_ext_nres f dec f1 f2 acc xs ys d \<equiv> doN {
+    (acc, xs, ys, stop) \<leftarrow> WHILEIT
+      (\<lambda>_. True)
+      (\<lambda>(acc, xs, ys, stop). xs \<noteq> [] \<and> ys \<noteq> [] \<and> \<not>stop)
+      (\<lambda>(acc, xs, ys, stop). doN {
+        ASSERT (xs \<noteq> [] \<and> ys \<noteq> []);
+        (x,xs) \<leftarrow> mop_list_pop_hd xs;
+        (y,ys) \<leftarrow> mop_list_pop_hd ys;
+        dir \<leftarrow> dec x y d;
+        acc \<leftarrow> f acc x y d dir;
+        if dir = STOP then RETURN (acc, xs, ys, True)
+        else if dir = LEFT then RETURN (acc, xs, y # ys, False)
+        else if dir = RIGHT then RETURN (acc, x # xs, ys, False)
+        else RETURN (acc, xs, ys, False)
+      })
+      (acc, xs, ys, False);
+    if stop then RETURN acc
+    else if ys = [] then foldl_nres f1 acc xs
+    else if xs = [] then foldl_nres f2 acc ys
+    else RETURN acc
+  }\<close>
+
+lemma ifoldl_ext_nres_refine:
+  assumes f: \<open>\<And>acc x y dir. fn acc x y d dir \<le> SPEC (\<lambda>r. r = f acc x y d dir)\<close>
+      and dec: \<open>\<And>x y. decn x y d \<le> SPEC (\<lambda>r. r = dec x y d)\<close>
+      and f1: \<open>\<And>acc x. f1n acc x \<le> SPEC (\<lambda>r. r = f1 acc x)\<close>
+      and f2: \<open>\<And>acc y. f2n acc y \<le> SPEC (\<lambda>r. r = f2 acc y)\<close>
+    shows \<open>ifoldl_ext_nres fn decn f1n f2n acc xs ys d
+      \<le> SPEC (\<lambda>r. r = ifoldl_ext f dec f1 f2 acc xs ys d)\<close>
+  unfolding ifoldl_ext_nres_def
+  apply (rule bind_rule)
+  apply (rule WHILEIT_true_rule[where
+        I = \<open>\<lambda>(acc', xs', ys', stop).
+              (if stop then acc' else ifoldl_ext f dec f1 f2 acc' xs' ys' d)
+                = ifoldl_ext f dec f1 f2 acc xs ys d\<close>
+        and R = \<open>measure (\<lambda>(acc', xs', ys', stop).
+              (if stop then 0 else length xs' + length ys' + 1))\<close>])
+  subgoal by simp
+  subgoal by simp
+  subgoal for s
+    apply (cases s rule: prod_cases4)
+    apply (simp only: prod.case)
+    apply (elim conjE)
+    apply (cases \<open>fst (snd s)\<close>; cases \<open>fst (snd (snd s))\<close>)
+    apply (simp_all add: mop_list_pop_hd_def)
+    apply (rule bind_rule)
+    apply (rule order_trans[OF dec])
+    apply (rule SPEC_rule)
+    apply (rule bind_rule)
+    apply (rule order_trans[OF f])
+    apply (rule SPEC_rule)
+    apply (auto split: direction.splits)
+    done
+  subgoal for s
+    apply (cases s rule: prod_cases4)
+    apply (auto simp: ifoldl_ext_Nil1 ifoldl_ext_Nil2 split: if_splits
+        intro: order_trans[OF foldl_nres_refine[OF f1]]
+               order_trans[OF foldl_nres_refine[OF f2]])
+    done
+  done
+
+
+subsection \<open>Unfolding equations for @{term ifoldl_ext_nres}\<close>
+
+lemma ifoldl_ext_nres_Nil2:
+  \<open>ifoldl_ext_nres fn decn f1n f2n acc xs [] d = foldl_nres f1n acc xs\<close>
+  unfolding ifoldl_ext_nres_def by (subst WHILEIT_unfold) simp
+
+lemma ifoldl_ext_nres_Nil1:
+  \<open>ifoldl_ext_nres fn decn f1n f2n acc [] ys d = foldl_nres f2n acc ys\<close>
+  unfolding ifoldl_ext_nres_def by (subst WHILEIT_unfold) (cases ys; simp)
+
+lemma ifoldl_ext_nres_Cons:
+  \<open>ifoldl_ext_nres fn decn f1n f2n acc (x # xs) (y # ys) d = doN {
+    dir \<leftarrow> decn x y d;
+    acc \<leftarrow> fn acc x y d dir;
+    case dir of
+      STOP \<Rightarrow> RETURN acc
+    | LEFT \<Rightarrow> ifoldl_ext_nres fn decn f1n f2n acc xs (y # ys) d
+    | RIGHT \<Rightarrow> ifoldl_ext_nres fn decn f1n f2n acc (x # xs) ys d
+    | BOTH \<Rightarrow> ifoldl_ext_nres fn decn f1n f2n acc xs ys d
+  }\<close>
+  unfolding ifoldl_ext_nres_def
+  apply (subst WHILEIT_unfold)
+  apply (simp add: mop_list_pop_hd_def)
+  apply (intro bind_cong[OF refl] ext)
+  apply (auto split: direction.splits)
+  text \<open>Remaining: the \<open>STOP\<close> case, where the loop exits at once.\<close>
+  apply (subst WHILEIT_unfold)
+  apply simp
+  done
+
+text \<open>@{term ifoldl_ext} with a constant extra argument is @{term ifoldl}
+  (and analogously for the monadic versions).\<close>
+
+lemma ifoldl_ext_ifoldl:
+  \<open>ifoldl_ext f dec f1 f2 acc xs ys d
+    = ifoldl (\<lambda>acc x y. f acc x y d) (\<lambda>x y. dec x y d) f1 f2 acc xs ys\<close>
+  by (induction f dec f1 f2 acc xs ys d rule: ifoldl_ext.induct)
+    (auto split: direction.splits)
+
+lemma ifoldl_ext_nres_ifoldl_nres:
+  \<open>ifoldl_ext_nres fn decn f1n f2n acc xs ys d
+    = ifoldl_nres (\<lambda>acc x y. fn acc x y d) (\<lambda>x y. decn x y d) f1n f2n acc xs ys\<close>
+  unfolding ifoldl_ext_nres_def ifoldl_nres_def ..
+
+section \<open>Implementation of @{term ifoldl_ext} for Copying Lists\<close>
+
+text \<open>Same loop as @{term cl_ifoldl}; the extra argument \<open>d\<close> is passed to
+  \<open>dec\<close> and \<open>f\<close> unchanged and is kept (never consumed) by both.\<close>
+
+definition cl_ifoldl_ext ::
+  \<open>('a::llvm_rep \<Rightarrow> 'b::llvm_rep \<Rightarrow> 'c::llvm_rep \<Rightarrow> 'd::llvm_rep \<Rightarrow> 8 word \<Rightarrow> 'a llM)
+    \<Rightarrow> ('b \<Rightarrow> 'c \<Rightarrow> 'd \<Rightarrow> 8 word llM)
+    \<Rightarrow> ('a \<Rightarrow> 'b \<Rightarrow> 'a llM) \<Rightarrow> ('a \<Rightarrow> 'c \<Rightarrow> 'a llM)
+    \<Rightarrow> 'a \<Rightarrow> 'b cl_list \<Rightarrow> 'c cl_list \<Rightarrow> 'd \<Rightarrow> 'a llM\<close>
+  where [llvm_code]:
+  \<open>cl_ifoldl_ext f dec f1 f2 acc xp yp d \<equiv> doM {
+    (acc, xp, yp, stop) \<leftarrow> llc_while cl_ifoldl_guard
+    (\<lambda>(acc, xp, yp, stop). doM {
+      xn \<leftarrow> ll_load xp;
+      yn \<leftarrow> ll_load yp;
+      let x = node.val xn;
+      let y = node.val yn;
+      dir \<leftarrow> dec x y d;
+      acc \<leftarrow> f acc x y d dir;
+      if dir = 0 then
+        Mreturn (acc, node.next xn, node.next yn, 1)
+      else if dir = 1 then
+        Mreturn (acc, node.next xn, yp, 0)
+      else if dir = 2 then
+        Mreturn (acc, xp, node.next yn, 0)
+      else
+        Mreturn (acc, node.next xn, node.next yn, 0)
+    }) (acc, xp, yp, 0 :: 1 word);
+    if to_bool stop then
+      Mreturn acc
+    else if yp = null then
+      cl_foldl_monadic' f1 (acc, xp)
+    else if xp = null then
+      cl_foldl_monadic' f2 (acc, yp)
+    else
+      Mreturn acc
+  }\<close>
+
+subsection \<open>Hoare rule for @{term cl_ifoldl_ext}\<close>
+
+lemma cl_ifoldl_ext_rule:
+  assumes F: \<open>\<And>a ai b bi c ci dr dri. llvm_htriple
+    (A a ai ** B b bi ** C c ci ** D d di ** dir_assn dr dri)
+    (fi ai bi ci di dri)
+    (\<lambda>r. A (f a b c d dr) r ** B b bi ** C c ci ** D d di)\<close>
+    and DEC: \<open>\<And>b bi c ci. llvm_htriple
+    (B b bi ** C c ci ** D d di)
+    (deci bi ci di)
+    (\<lambda>r. dir_assn (dec b c d) r ** B b bi ** C c ci ** D d di)\<close>
+    and F1: \<open>\<And>a ai b bi. llvm_htriple
+    (A a ai ** B b bi)
+    (f1i ai bi)
+    (\<lambda>r. A (f1 a b) r ** B b bi)\<close>
+    and F2: \<open>\<And>a ai c ci. llvm_htriple
+    (A a ai ** C c ci)
+    (f2i ai ci)
+    (\<lambda>r. A (f2 a c) r ** C c ci)\<close>
+  shows \<open>llvm_htriple
+    (A acc acci ** cl_assn' B bs bsi ** cl_assn' C cs csi ** D d di)
+    (cl_ifoldl_ext fi deci f1i f2i acci bsi csi di)
+    (\<lambda>r. A (ifoldl_ext f dec f1 f2 acc bs cs d) r
+      ** cl_assn' B bs bsi ** cl_assn' C cs csi ** D d di)\<close>
+proof -
+  interpret llvm_prim_ctrl_setup .
+  show ?thesis
+  unfolding cl_ifoldl_ext_def
+  apply (rewrite annotate_llc_while [where
+    I = \<open>\<lambda>(acci', xp, yp, stop) t. EXS i j acc'.
+        A acc' acci'
+        ** olseg B (take i bs) bsi xp ** olseg C (take j cs) csi yp
+        ** cl_assn' B (drop i bs) xp ** cl_assn' C (drop j cs) yp
+        ** D d di
+        ** \<up>((if stop = 0
+               then ifoldl_ext f dec f1 f2 acc' (drop i bs) (drop j cs) d
+               else acc')
+              = ifoldl_ext f dec f1 f2 acc bs cs d)
+        ** \<up>\<^sub>!(t = (if stop = 0 then Suc (length bs - i + (length cs - j)) else 0))\<close>
+    and R = \<open>measure id\<close>])
+  supply [vcg_rules] = F DEC ll_icmp_eq_bool_rule cl_assn'_load_rule
+    cl_fold_monadic'_rule[where A=A and B=B and fi=f1i and f=f1, OF F1]
+    cl_fold_monadic'_rule[where A=A and B=C and fi=f2i and f=f2, OF F2]
+  supply [simp] = cl_assn_simps olseg_nil sep_conj_exists drop_head
+    hd_drop_conv_nth drop_Suc[symmetric] ifoldl_ext_Nil1 ifoldl_ext_Nil2
+  supply [fri_rules] = cl_assn'_cong_fri olseg_empty_fri olseg_cl_fri
+  supply [fri_red_rules] = olseg_snoc_red olseg_cl_reassemble_red cl_assn'_cons_red
+  apply vcg_monadify
+  apply vcg'
+  subgoal for aa ab x xa
+    by (cases \<open>dec (bs ! x) (cs ! xa) d\<close>) auto
+  done
+qed
+
+subsection \<open>Refinement rule for @{term cl_ifoldl_ext} against @{term ifoldl_ext_nres}\<close>
+
+lemma cl_ifoldl_ext_nres_rule:
+  assumes F: \<open>\<And>a ai b bi c ci dr dri. nofail (fn a b c d dr) \<Longrightarrow> llvm_htriple
+    (A a ai ** B b bi ** C c ci ** D d di ** dir_assn dr dri)
+    (fi ai bi ci di dri)
+    (\<lambda>r. B b bi ** C c ci ** D d di ** (EXS x. A x r ** \<up>(RETURN x \<le> fn a b c d dr)))\<close>
+    and DEC: \<open>\<And>b bi c ci. nofail (decn b c d) \<Longrightarrow> llvm_htriple
+    (B b bi ** C c ci ** D d di)
+    (deci bi ci di)
+    (\<lambda>r. B b bi ** C c ci ** D d di ** (EXS dr. dir_assn dr r ** \<up>(RETURN dr \<le> decn b c d)))\<close>
+    and F1: \<open>\<And>a ai b bi. nofail (f1n a b) \<Longrightarrow> llvm_htriple
+    (A a ai ** B b bi)
+    (f1i ai bi)
+    (\<lambda>r. B b bi ** (EXS x. A x r ** \<up>(RETURN x \<le> f1n a b)))\<close>
+    and F2: \<open>\<And>a ai c ci. nofail (f2n a c) \<Longrightarrow> llvm_htriple
+    (A a ai ** C c ci)
+    (f2i ai ci)
+    (\<lambda>r. C c ci ** (EXS x. A x r ** \<up>(RETURN x \<le> f2n a c)))\<close>
+    and NF: \<open>nofail (ifoldl_ext_nres fn decn f1n f2n acc bs cs d)\<close>
+  shows \<open>llvm_htriple
+    (A acc acci ** cl_assn' B bs bsi ** cl_assn' C cs csi ** D d di)
+    (cl_ifoldl_ext fi deci f1i f2i acci bsi csi di)
+    (\<lambda>r. cl_assn' B bs bsi ** cl_assn' C cs csi ** D d di
+      ** (EXS x. A x r ** \<up>(RETURN x \<le> ifoldl_ext_nres fn decn f1n f2n acc bs cs d)))\<close>
+proof -
+  interpret llvm_prim_ctrl_setup .
+  show ?thesis
+  using NF
+  unfolding cl_ifoldl_ext_def
+  apply (rewrite annotate_llc_while [where
+    I = \<open>\<lambda>(acci', xp, yp, stop) t. EXS i j acc'.
+        A acc' acci'
+        ** olseg B (take i bs) bsi xp ** olseg C (take j cs) csi yp
+        ** cl_assn' B (drop i bs) xp ** cl_assn' C (drop j cs) yp
+        ** D d di
+        ** \<up>((if stop = 0
+               then ifoldl_ext_nres fn decn f1n f2n acc' (drop i bs) (drop j cs) d
+               else RETURN acc')
+              \<le> ifoldl_ext_nres fn decn f1n f2n acc bs cs d)
+        ** \<up>\<^sub>!(t = (if stop = 0 then Suc (length bs - i + (length cs - j)) else 0))\<close>
+    and R = \<open>measure id\<close>])
+  supply [vcg_rules] = F DEC ll_icmp_eq_bool_rule cl_assn'_load_rule
+    cl_fold_monadic'_nres_rule'[where A=A and B=B and fi=f1i and f=f1n, OF F1]
+    cl_fold_monadic'_nres_rule'[where A=A and B=C and fi=f2i and f=f2n, OF F2]
+  supply [simp] = cl_assn_simps olseg_nil sep_conj_exists drop_head
+    hd_drop_conv_nth drop_Suc[symmetric]
+    ifoldl_ext_nres_Nil1 ifoldl_ext_nres_Nil2 ifoldl_ext_nres_Cons
+    pw_le_iff refine_pw_simps
+  supply [fri_rules] = cl_assn'_cong_fri olseg_empty_fri olseg_cl_fri
+  supply [fri_red_rules] = olseg_snoc_red olseg_cl_reassemble_red cl_assn'_cons_red
+  apply vcg_monadify
+  apply vcg'
+  apply (auto split: direction.splits)
+  subgoal by blast
+  subgoal by blast
+  subgoal by blast
+  subgoal by (meson direction.exhaust)
+  subgoal by metis
+  done
+qed
+
+subsection \<open>hfref forms for @{term cl_ifoldl_ext}\<close>
+
+lemma hfref_nres_htriple_d1_k2_k3_k4_k5:
+  assumes R: \<open>(uncurry4 fi, uncurry4 fn)
+      \<in> A\<^sup>d *\<^sub>a B\<^sup>k *\<^sub>a C\<^sup>k *\<^sub>a D\<^sup>k *\<^sub>a dir_assn\<^sup>k \<rightarrow>\<^sub>a A\<close>
+    and NF: \<open>nofail (fn a b c d dr)\<close>
+  shows \<open>llvm_htriple (A a ai ** B b bi ** C c ci ** D d di ** dir_assn dr dri)
+    (fi ai bi ci di dri)
+    (\<lambda>r. B b bi ** C c ci ** D d di ** (EXS x. A x r ** \<up>(RETURN x \<le> fn a b c d dr)))\<close>
+proof -
+  note HT = R[to_hnr, unfolded autoref_tag_defs, THEN hn_refineD, OF NF]
+  show ?thesis
+    apply (rule htriple_ent_pre[OF _ htriple_ent_post[OF _ HT]])
+    unfolding hn_ctxt_def
+    subgoal by (rule entails_refl)
+    subgoal
+      by (auto simp: entails_def sep_algebra_simps sep_conj_exists invalid_assn_def
+          pred_lift_extract_simps)
+    done
+qed
+
+lemma hfref_nres_htriple_k1_k2_k3:
+  assumes R: \<open>(uncurry2 fi, uncurry2 fn) \<in> B\<^sup>k *\<^sub>a C\<^sup>k *\<^sub>a D\<^sup>k \<rightarrow>\<^sub>a E\<close>
+    and NF: \<open>nofail (fn b c d)\<close>
+  shows \<open>llvm_htriple (B b bi ** C c ci ** D d di) (fi bi ci di)
+    (\<lambda>r. B b bi ** C c ci ** D d di ** (EXS x. E x r ** \<up>(RETURN x \<le> fn b c d)))\<close>
+proof -
+  note HT = R[to_hnr, unfolded autoref_tag_defs, THEN hn_refineD, OF NF]
+  show ?thesis
+    apply (rule htriple_ent_pre[OF _ htriple_ent_post[OF _ HT]])
+    unfolding hn_ctxt_def
+    subgoal by (rule entails_refl)
+    subgoal
+      by (auto simp: entails_def sep_algebra_simps sep_conj_exists
+          pred_lift_extract_simps)
+    done
+qed
+
+lemma cl_ifoldl_ext_nres_hfref:
+  assumes F: \<open>(uncurry4 fi, uncurry4 fn)
+      \<in> A\<^sup>d *\<^sub>a B\<^sup>k *\<^sub>a C\<^sup>k *\<^sub>a D\<^sup>k *\<^sub>a dir_assn\<^sup>k \<rightarrow>\<^sub>a A\<close>
+    and DEC: \<open>(uncurry2 deci, uncurry2 decn) \<in> B\<^sup>k *\<^sub>a C\<^sup>k *\<^sub>a D\<^sup>k \<rightarrow>\<^sub>a dir_assn\<close>
+    and F1: \<open>(uncurry f1i, uncurry f1n) \<in> A\<^sup>d *\<^sub>a B\<^sup>k \<rightarrow>\<^sub>a A\<close>
+    and F2: \<open>(uncurry f2i, uncurry f2n) \<in> A\<^sup>d *\<^sub>a C\<^sup>k \<rightarrow>\<^sub>a A\<close>
+  shows \<open>(uncurry3 (cl_ifoldl_ext fi deci f1i f2i), uncurry3 (ifoldl_ext_nres fn decn f1n f2n))
+    \<in> A\<^sup>d *\<^sub>a (cl_assn' B)\<^sup>k *\<^sub>a (cl_assn' C)\<^sup>k *\<^sub>a D\<^sup>k \<rightarrow>\<^sub>a A\<close>
+  supply [vcg_rules] = cl_ifoldl_ext_nres_rule[where A=A and B=B and C=C and D=D
+      and fi=fi and deci=deci and f1i=f1i and f2i=f2i
+      and fn=fn and decn=decn and f1n=f1n and f2n=f2n,
+      OF hfref_nres_htriple_d1_k2_k3_k4_k5[OF F] hfref_nres_htriple_k1_k2_k3[OF DEC]
+         hfref_nres_htriple_d1_k2[OF F1] hfref_nres_htriple_d1_k2[OF F2]]
+  by (sepref_to_hoare; vcg)
+
+lemma cl_ifoldl_ext_hfref:
+  assumes F: \<open>(uncurry4 fi, uncurry4 (RETURN ooooo f))
+      \<in> A\<^sup>d *\<^sub>a B\<^sup>k *\<^sub>a C\<^sup>k *\<^sub>a D\<^sup>k *\<^sub>a dir_assn\<^sup>k \<rightarrow>\<^sub>a A\<close>
+    and DEC: \<open>(uncurry2 deci, uncurry2 (RETURN ooo dec))
+      \<in> B\<^sup>k *\<^sub>a C\<^sup>k *\<^sub>a D\<^sup>k \<rightarrow>\<^sub>a dir_assn\<close>
+    and F1: \<open>(uncurry f1i, uncurry (RETURN oo f1)) \<in> A\<^sup>d *\<^sub>a B\<^sup>k \<rightarrow>\<^sub>a A\<close>
+    and F2: \<open>(uncurry f2i, uncurry (RETURN oo f2)) \<in> A\<^sup>d *\<^sub>a C\<^sup>k \<rightarrow>\<^sub>a A\<close>
+  shows \<open>(uncurry3 (cl_ifoldl_ext fi deci f1i f2i),
+          uncurry3 (RETURN oooo ifoldl_ext f dec f1 f2))
+    \<in> A\<^sup>d *\<^sub>a (cl_assn' B)\<^sup>k *\<^sub>a (cl_assn' C)\<^sup>k *\<^sub>a D\<^sup>k \<rightarrow>\<^sub>a A\<close>
+proof -
+  note M = cl_ifoldl_ext_nres_hfref[OF F DEC F1 F2]
+  have LE: \<open>ifoldl_ext_nres (RETURN ooooo f) (RETURN ooo dec) (RETURN oo f1) (RETURN oo f2)
+      acc bs cs d \<le> RETURN (ifoldl_ext f dec f1 f2 acc bs cs d)\<close> for acc bs cs d
+    by (rule order_trans[OF ifoldl_ext_nres_refine]) (simp_all add: pw_le_iff refine_pw_simps)
+  show ?thesis
+    apply (rule hfrefI)
+    apply (rule hn_refine_ref[OF _ hfrefD[OF M]])
+    by (auto simp: LE)
+qed
 
 experiment
 begin
@@ -772,6 +1130,46 @@ definition \<open>test \<equiv> ifoldl ftest dirtest f1test f2test []\<close>
 sepref_def test_impl is \<open>uncurry (RETURN oo test)\<close>
   :: \<open>(cl_assn' u8_assn)\<^sup>k *\<^sub>a (cl_assn' u8_assn)\<^sup>k \<rightarrow>\<^sub>a cl_assn' u8_assn\<close>
   unfolding test_def test_ifoldl_def[symmetric]
+  by sepref
+
+
+text \<open>Extended version: the extra argument is an owning list, kept throughout.\<close>
+definition \<open>ftest_ext a b c d dir \<equiv>
+  if dir = STOP then a
+  else if dir = LEFT then c # b # a
+  else if dir = RIGHT then b # c # a
+  else if d = [] then a else b # a
+\<close>
+sepref_def ftest_ext_impl is \<open>uncurry4 (RETURN ooooo ftest_ext)\<close>
+  :: \<open>(cl_assn' u8_assn)\<^sup>d *\<^sub>a u8_assn\<^sup>k *\<^sub>a u8_assn\<^sup>k *\<^sub>a (cl_assn' u8_assn)\<^sup>k
+      *\<^sub>a dir_assn\<^sup>k \<rightarrow>\<^sub>a (cl_assn' u8_assn)\<close>
+  unfolding ftest_ext_def ls_emp'
+  by sepref
+
+definition \<open>dirtest_ext a b d \<equiv>
+  if d = [] then STOP
+  else if a = b then BOTH
+  else if a < b then LEFT
+  else RIGHT
+\<close>
+sepref_def dirtest_ext_impl is \<open>uncurry2 (RETURN ooo dirtest_ext)\<close>
+  :: \<open>u8_assn\<^sup>k *\<^sub>a u8_assn\<^sup>k *\<^sub>a (cl_assn' u8_assn)\<^sup>k \<rightarrow>\<^sub>a dir_assn\<close>
+  unfolding dirtest_ext_def ls_emp'
+  by sepref
+
+definition \<open>test_ifoldl_ext \<equiv> ifoldl_ext ftest_ext dirtest_ext f1test f2test\<close>
+sepref_register test_ifoldl_ext
+
+lemmas test_ifoldl_ext_hnr[sepref_fr_rules] =
+  cl_ifoldl_ext_hfref[OF ftest_ext_impl.refine dirtest_ext_impl.refine
+    f1test_impl.refine f2test_impl.refine, folded test_ifoldl_ext_def]
+
+definition \<open>test_ext xs ys d \<equiv> ifoldl_ext ftest_ext dirtest_ext f1test f2test [] xs ys d\<close>
+
+sepref_def test_ext_impl is \<open>uncurry2 (RETURN ooo test_ext)\<close>
+  :: \<open>(cl_assn' u8_assn)\<^sup>k *\<^sub>a (cl_assn' u8_assn)\<^sup>k *\<^sub>a (cl_assn' u8_assn)\<^sup>k
+      \<rightarrow>\<^sub>a cl_assn' u8_assn\<close>
+  unfolding test_ext_def test_ifoldl_ext_def[symmetric]
   by sepref
 
 end
